\documentclass{article}
\usepackage[utf8]{inputenc}
\usepackage{amsmath, amssymb, bm}
\usepackage{gensymb}

\begin{document}
	\textbf{Theorem 1.4.4:} Let $f$ and $g$ be real-valued functions and $L$ and $M$ be real numbers. Suppose that
	$$\lim_{x \to a}{f(x)} = L \; \text{ and } \lim_{x \to a}{g(x)} = M$$
	Then
	$$\lim_{x \to a}[{f(x) - g(x)}] = L - M.$$
	\textbf{Proof:}
	\begin{align*}
		\lim_{x \to a}[{f(x) - g(x)}] &= \lim_{x \to a}[{f(x) + (-1) * g(x)}] \\
									  &= \lim_{x \to a}{f(x)} + \lim_{x \to a}{[(-1) * g(x)]} \tag{Theorem 1.4.1} \\
									  &= L + (-1) * \lim_{x \to a}{g(x)} \tag{Theorem 1.4.3} \\
									  &= L + (-1) * M \\
									  &= L - M.
	\end{align*}
\end{document}