\documentclass{article}
\usepackage[utf8]{inputenc}
\usepackage{amsmath, amssymb, bm}
\usepackage{gensymb}

\begin{document}
	\textbf{Theorem 1.4.8:} Let $f$ be a polynomial and $b \in \mathbb{R}$. Then
	$$\lim_{x \to b}{f(x)} = f(b).$$
	\textbf{Proof:}
	Let $f$ be an arbitrary polynomial. We will proceed by induction. \\\\
	\textit{Step 1: Base case} \\
	Let $\deg{[f(x)]} = 0$. Then
	$$f(x) = a_0$$
	So
	\begin{align*}
		\lim_{x \to b}{f(x)} &= \lim_{x \to b}{a_0} \\
		                     &= a_0 \tag{Theorem 1.3.3} \\
		                     &= f(b)
	\end{align*}
	So the statement holds for the base case. \\\\
	\textit{Step 2: Induction step} \\
	Let $\deg{[f(x)] = n}$ and suppose $\lim_{x \to b}{f(x)} = f(b)$. Let $g$ be an arbitrary polynomial of degree $n + 1$. We then need to show that
	$$\lim_{x \to b}{g(x)} = g(b)$$
	We have
	\begin{align*}
		\lim_{x \to b}{g(x)} &= \lim_{x \to b}{\left[a_{n+1}x^{n+1} + a_nx^n + a_{n-1}x^{n-1} + \ldots + a_2x^2 + a_1x + a_0\right]} \\
		                     &= \lim_{x \to b}{\left[a_{n+1}x^{n+1}\right] + \lim_{x \to b}\left[a_nx^n + a_{n-1}x^{n-1} + \ldots + a_2x^2 + a_1x + a_0\right]} \tag{Theorem 1.4.1} \\
		                     &=  \lim_{x \to b}{\left[a_{n+1}x^{n+1}\right]} + \lim_{x \to b}{f(x)}\\
		                     &= a_{n+1} * \lim_{x \to b}{x^{n+1}} + f(b) \tag{Theorem 1.4.3}\\
		                     &= a_{n+1}b^{n+1} + f(b) \tag{Theorem 1.4.7}\\
		                     &= a_{n+1}b^{n+1} + a_nb^n + a_{n-1}b^{n-1} + \ldots + a_2b^2 + a_1b + a_0 \\
		                     &= g(b)
	\end{align*}
	which is what we needed to show.
	
	We have proven the base case and the induction step. Thus, by the principle of mathematical induction, the statement
	$$\lim_{x \to b}{f(x)} = f(b)$$
	holds for polynomials of any degree $n \geq 0$.
	 
\end{document}